Revert some bad modification. It is still a broken commit.

SeparationLogic/ProofTheory/SeparationLogic.v
@@ -24,35 +24,21 @@ Class SeparationLogic (L: Language) {nL: NormalLanguage L} {pL: PropositionalLan
   sepcon_mono: forall x1 x2 y1 y2, |-- x1 --> x2 -> |-- y1 --> y2 -> |-- (x1 * y1) --> (x2 * y2)
 }.
 
-Class SeparationEmpLogic (L: Language) {nL: NormalLanguage L} {pL: PropositionalLanguage L} {sL: SeparationLanguage L} {s'L: SeparationEmpLanguage L} (Gamma: ProofTheory L) {nGamma: NormalProofTheory L Gamma} {mpGamma: MinimunPropositionalLogic L Gamma} {ipGamma: IntuitionisticPropositionalLogic L Gamma} {sGamma: SeparationLogic L Gamma} := {
-  sepcon_emp_l: forall x, |-- x * emp --> x
+Class EmpSeparationLogic (L: Language) {nL: NormalLanguage L} {pL: PropositionalLanguage L} {sL: SeparationLanguage L} {s'L: SeparationEmpLanguage L} (Gamma: ProofTheory L) {nGamma: NormalProofTheory L Gamma} {mpGamma: MinimunPropositionalLogic L Gamma} {ipGamma: IntuitionisticPropositionalLogic L Gamma} {sGamma: SeparationLogic L Gamma} := {
+  sepcon_emp: forall x, |-- x * emp <--> x
 }.
 
 Class ExtSeparationLogic (L: Language) {nL: NormalLanguage L} {pL: PropositionalLanguage L} {sL: SeparationLanguage L} (Gamma: ProofTheory L) {nGamma: NormalProofTheory L Gamma} {mpGamma: MinimunPropositionalLogic L Gamma} {ipGamma: IntuitionisticPropositionalLogic L Gamma} {sGamma: SeparationLogic L Gamma} := {
   sepcon_ext: forall x, |-- x --> x * TT
 }.
 
-Class GarbageCollectSeparationLogic (L: Language) {nL: NormalLanguage L} {pL: PropositionalLanguage L} {sL: SeparationLanguage L} (Gamma: ProofTheory L) {nGamma: NormalProofTheory L Gamma} {mpGamma: MinimunPropositionalLogic L Gamma} {ipGamma: IntuitionisticPropositionalLogic L Gamma} {sGamma: SeparationLogic L Gamma} := {
-  sepcon_elim1: forall x y, |-- x * y --> x
-}.
-
-Class UnitalSeparationLogic (L: Language) {nL: NormalLanguage L} {pL: PropositionalLanguage L} {sL: SeparationLanguage L} {s'L: SeparationEmpLanguage L} (Gamma: ProofTheory L) {nGamma: NormalProofTheory L Gamma} {mpGamma: MinimunPropositionalLogic L Gamma} {ipGamma: IntuitionisticPropositionalLogic L Gamma} {sGamma: SeparationLogic L Gamma} {eGamma: SeparationEmpLogic L Gamma} := {
-  sepcon_emp_r: forall x, |-- x --> x * emp
-}.
-
-Class NonsplitEmpSeparationLogic (L: Language) {nL: NormalLanguage L} {pL: PropositionalLanguage L} {sL: SeparationLanguage L} {s'L: SeparationEmpLanguage L} (Gamma: ProofTheory L) {nGamma: NormalProofTheory L Gamma} {mpGamma: MinimunPropositionalLogic L Gamma} {ipGamma: IntuitionisticPropositionalLogic L Gamma} {sGamma: SeparationLogic L Gamma} {eGamma: SeparationEmpLogic L Gamma} := {
-  emp_sepcon_elim1: forall x y, |-- x * y && emp --> x
-}.
-
-Class DupEmpSeparationLogic (L: Language) {nL: NormalLanguage L} {pL: PropositionalLanguage L} {sL: SeparationLanguage L} {s'L: SeparationEmpLanguage L} (Gamma: ProofTheory L) {nGamma: NormalProofTheory L Gamma} {mpGamma: MinimunPropositionalLogic L Gamma} {ipGamma: IntuitionisticPropositionalLogic L Gamma} {sGamma: SeparationLogic L Gamma} := {
+Class MallocFreeSeparationLogic (L: Language) {nL: NormalLanguage L} {pL: PropositionalLanguage L} {sL: SeparationLanguage L} {s'L: SeparationEmpLanguage L} (Gamma: ProofTheory L) {nGamma: NormalProofTheory L Gamma} {mpGamma: MinimunPropositionalLogic L Gamma} {ipGamma: IntuitionisticPropositionalLogic L Gamma} {sGamma: SeparationLogic L Gamma} := {
+  emp_sepcon_elim1: forall x y, |-- x * y && emp --> x;
   emp_dup: forall x, |-- x && emp --> x * x
 }.
 
-Class MallocFreeSeparationLogic (L: Language) {nL: NormalLanguage L} {pL: PropositionalLanguage L} {sL: SeparationLanguage L} {s'L: SeparationEmpLanguage L} (Gamma: ProofTheory L) {nGamma: NormalProofTheory L Gamma} {mpGamma: MinimunPropositionalLogic L Gamma} {ipGamma: IntuitionisticPropositionalLogic L Gamma} {sGamma: SeparationLogic L Gamma} {eGamma: SeparationEmpLogic L Gamma} := {
-  MallocFreeSeparationLogic_NonsplitEmpSeparationLogic :>
-    NonsplitEmpSeparationLogic L Gamma;
-  MallocFreeSeparationLogic_DupEmpSeparationLogic :>
-    DupEmpSeparationLogic L Gamma
+Class GarbageCollectSeparationLogic (L: Language) {nL: NormalLanguage L} {pL: PropositionalLanguage L} {sL: SeparationLanguage L} (Gamma: ProofTheory L) {nGamma: NormalProofTheory L Gamma} {mpGamma: MinimunPropositionalLogic L Gamma} {ipGamma: IntuitionisticPropositionalLogic L Gamma} {sGamma: SeparationLogic L Gamma} := {
+  sepcon_elim1: forall x y, |-- x * y --> x
 }.
 
 Lemma derivable_sepcon_comm: forall {L: Language} {nL: NormalLanguage L} {pL: PropositionalLanguage L} {sL: SeparationLanguage L} {Gamma: ProofTheory L} {nGamma: NormalProofTheory L Gamma} {mpGamma: MinimunPropositionalLogic L Gamma} {ipGamma: IntuitionisticPropositionalLogic L Gamma} {sGamma: SeparationLogic L Gamma} (Phi: context) (x y: expr),
@@ -71,19 +57,11 @@ Proof.
   apply deduction_weaken0; auto.
 Qed.
 
-Lemma derivable_sepcon_emp_l: forall {L: Language} {nL: NormalLanguage L} {pL: PropositionalLanguage L} {sL: SeparationLanguage L} {s'L: SeparationEmpLanguage L} {Gamma: ProofTheory L} {nGamma: NormalProofTheory L Gamma} {mpGamma: MinimunPropositionalLogic L Gamma} {ipGamma: IntuitionisticPropositionalLogic L Gamma} {sGamma: SeparationLogic L Gamma} {eGamma: SeparationEmpLogic L Gamma} (Phi: context) (x: expr),
-  Phi |-- x * emp --> x.
+Lemma derivable_sepcon_emp: forall {L: Language} {nL: NormalLanguage L} {pL: PropositionalLanguage L} {sL: SeparationLanguage L} {s'L: SeparationEmpLanguage L} {Gamma: ProofTheory L} {nGamma: NormalProofTheory L Gamma} {mpGamma: MinimunPropositionalLogic L Gamma} {ipGamma: IntuitionisticPropositionalLogic L Gamma} {sGamma: SeparationLogic L Gamma} {EmpsGamma: EmpSeparationLogic L Gamma} (Phi: context) (x: expr),
+  Phi |-- x * emp <--> x.
 Proof.
   intros.
-  pose proof sepcon_emp_l x.
-  apply deduction_weaken0; auto.
-Qed.
-
-Lemma derivable_sepcon_emp_r: forall {L: Language} {nL: NormalLanguage L} {pL: PropositionalLanguage L} {sL: SeparationLanguage L} {s'L: SeparationEmpLanguage L} {Gamma: ProofTheory L} {nGamma: NormalProofTheory L Gamma} {mpGamma: MinimunPropositionalLogic L Gamma} {ipGamma: IntuitionisticPropositionalLogic L Gamma} {sGamma: SeparationLogic L Gamma} {eGamma: SeparationEmpLogic L Gamma} {ueGamma: UnitalSeparationLogic L Gamma} (Phi: context) (x: expr),
-  Phi |-- x --> x * emp.
-Proof.
-  intros.
-  pose proof sepcon_emp_r x.
+  pose proof sepcon_emp x.
   apply deduction_weaken0; auto.
 Qed.
 
@@ -132,4 +110,3 @@ Proof.
   apply deduction_weaken0.
   apply sepcon_comm.
 Qed.
-
